characteristic/cfFFITypeScript.sml
@@ -1,0 +1,270 @@
+open preamble;
+
+val _ = new_theory "cfFFIType"
+
+(*
+
+This file defines a tyep (abbreviation) that behaves like the
+following type:
+
+val _ = Datatype `
+  ffi = Str string
+      | Num num
+      | Cons ffi ffi
+      | List (ffi list)
+      | Stream (num llist)
+      | Seq (num -> ffi)
+
+The type is missing a cases thm and an ind thm.
+
+*)
+
+val _ = Datatype `
+  inner_ffi = iNum num
+            | iStr string
+            | iStream (num llist)`
+
+val _ = type_abbrev("ffi",``:num -> inner_ffi``)
+
+(* constructors *)
+
+val Num_def = Define `
+  ((Num i):ffi) =
+    \n. if n = 0 then iNum 0 else iNum i`
+
+val Str_def = Define `
+  ((Str i):ffi) =
+    \n. if n = 0 then iNum 1 else iStr i`
+
+val Cons_def = Define `
+  ((Cons (x:ffi) (y:ffi)):ffi) =
+    \n. if n = 0 then iNum 2 else
+          let n = n - 1 in
+            if EVEN n then x (n DIV 2) else y (n DIV 2)`
+
+val List_def = Define `
+  ((List (xs:ffi list)):ffi) =
+    \n. if n = 0 then iNum 3 else FOLDR Cons (Num 0) xs (n-1) `
+
+val Stream_def = Define `
+  ((Stream i):ffi) =
+    \n. if n = 0 then iNum 4 else iStream i`
+
+val factor_count_def = Define `
+  factor_count k n =
+    if k <= 1 then 0n else
+    if n = 0n then 0 else
+    if n MOD k = 0 then 1 + factor_count k (n DIV k) else 0`
+
+val Seq_def = Define `
+  ((Seq (f:num -> ffi)):ffi) =
+    \n. if n = 0 then iNum 5 else
+          let n = n - 1 in
+            f (factor_count 2 n) (factor_count 3 n)`;
+
+(* injectivity *)
+
+val Num_11 = store_thm("Num_11[simp]",
+  ``!n1 n2. Num n1 = Num n2 <=> n1 = n2``,
+  fs [Num_def,FUN_EQ_THM]
+  \\ rw [] \\ eq_tac \\ rw []
+  \\ pop_assum (qspec_then `1` mp_tac) \\ fs []);
+
+val Str_11 = store_thm("Str_11[simp]",
+  ``!n1 n2. Str n1 = Str n2 <=> n1 = n2``,
+  fs [Str_def,FUN_EQ_THM]
+  \\ rw [] \\ eq_tac \\ rw []
+  \\ pop_assum (qspec_then `1` mp_tac) \\ fs []);
+
+val Cons_11 = store_thm("Cons_11[simp]",
+  ``!x1 x2 y1 y2. Cons x1 x2 = Cons y1 y2 <=> x1 = y1 /\ x2 = y2``,
+  fs [Cons_def,FUN_EQ_THM]
+  \\ rw [] \\ eq_tac \\ rw []
+  THEN1
+   (pop_assum (qspec_then `2 * x + 1` mp_tac) \\ fs []
+    \\ fs [FUN_EQ_THM,EVEN_DOUBLE]
+    \\ once_rewrite_tac [MULT_COMM]
+    \\ simp [MULT_DIV,DIV_MULT] \\ rw [])
+  THEN1
+   (pop_assum (qspec_then `2 * x + 2` mp_tac) \\ fs []
+    \\ fs [FUN_EQ_THM,EVEN_DOUBLE]
+    \\ once_rewrite_tac [MULT_COMM]
+    \\ simp [MULT_DIV,DIV_MULT] \\ rw []
+    \\ fs [EVEN_ODD,GSYM ADD1,ODD_DOUBLE]));
+
+val Cons_NOT_Num = prove(
+  ``Cons x y <> Num z``,
+  fs [FUN_EQ_THM] \\ qexists_tac `0` \\ EVAL_TAC);
+
+val List_11 = store_thm("List_11[simp]",
+  ``!xs ys. List xs = List ys <=> xs = ys``,
+  rw [] \\ eq_tac \\ rw []
+  \\ fs [List_def,FUN_EQ_THM]
+  \\ pop_assum (mp_tac o Q.GEN `n` o Q.SPEC `n+1`)
+  \\ fs [GSYM FUN_EQ_THM]
+  \\ CONV_TAC (DEPTH_CONV ETA_CONV)
+  \\ qspec_tac (`ys`,`ys`)
+  \\ Induct_on `xs` \\ Cases_on `ys` \\ fs [Cons_NOT_Num]);
+
+val Stream_11 = store_thm("Stream_11[simp]",
+  ``!n1 n2. Stream n1 = Stream n2 <=> n1 = n2``,
+  fs [Stream_def,FUN_EQ_THM]
+  \\ rw [] \\ eq_tac \\ rw []
+  \\ pop_assum (qspec_then `1` mp_tac) \\ fs []);
+
+val factor_count_2 = prove(
+  ``!m n. factor_count 2 (2 ** m * 3 ** n) = m``,
+  Induct \\ once_rewrite_tac [factor_count_def] \\ fs []
+  \\ fs [EXP,ADD1] \\ once_rewrite_tac [MULT_COMM] \\ fs [MULT_DIV]);
+
+val factor_count_3 = prove(
+  ``!m n. factor_count 3 (3 ** m * 2 ** n) = m``,
+  Induct \\ once_rewrite_tac [factor_count_def] \\ fs []
+  \\ fs [EXP,ADD1] \\ once_rewrite_tac [MULT_COMM] \\ fs [MULT_DIV]
+  \\ rw [] \\ pop_assum mp_tac \\ fs []
+  \\ Induct_on `n` \\ fs [EXP]
+  \\ once_rewrite_tac [GSYM (MATCH_MP MOD_TIMES2 (DECIDE ``0<3n``))]
+  \\ Cases_on `2 ** n MOD 3` \\ fs []
+  \\ Cases_on `n'` \\ fs []
+  \\ Cases_on `n''` \\ fs []
+  \\ `2 ** n MOD 3 < 3` by fs []
+  \\ rev_full_simp_tac bool_ss [] \\ fs [ADD1]);
+
+val Seq_11 = store_thm("Seq_11[simp]",
+  ``Seq f1 = Seq f2 <=> f1 = f2``,
+  eq_tac \\ rw [] \\ fs [FUN_EQ_THM,Seq_def] \\ rw []
+  \\ pop_assum (qspec_then `2 ** x * 3 ** x' + 1` mp_tac)
+  \\ fs [factor_count_3,factor_count_2]
+  \\ once_rewrite_tac [MULT_COMM]
+  \\ fs [factor_count_3,factor_count_2]);
+
+(* distinctness *)
+
+val ffi_distinct = prove(
+  ``ALL_DISTINCT [Num n; Str s; Cons x y; List l; Stream ll; Seq f]``,
+  rw [] \\ fs [FUN_EQ_THM] \\ qexists_tac `0` \\ EVAL_TAC)
+  |> SIMP_RULE std_ss [ALL_DISTINCT,MEM,GSYM CONJ_ASSOC] |> GEN_ALL
+  |> curry save_thm "ffi_distinct[simp]";
+
+(* destructors *)
+
+val destNum_def = new_specification("destNum_def",["destNum"],prove(``
+  ?destNum.
+    (!n. destNum (Num n) = SOME n) /\
+    (!s. destNum (Str s) = NONE) /\
+    (!x y. destNum (Cons x y) = NONE) /\
+    (!l. destNum (List l) = NONE) /\
+    (!ll. destNum (Stream ll) = NONE) /\
+    (!f. destNum (Seq f) = NONE)``,
+  qexists_tac `\f. if f 0 = iNum 0 then SOME (@n. Num n = f) else NONE`
+  \\ fs [] \\ rw [] \\ EVAL_TAC));
+val _ = export_rewrites ["destNum_def"];
+
+val destStr_def = new_specification("destStr_def",["destStr"],prove(``
+  ?destStr.
+    (!n. destStr (Num n) = NONE) /\
+    (!s. destStr (Str s) = SOME s) /\
+    (!x y. destStr (Cons x y) = NONE) /\
+    (!l. destStr (List l) = NONE) /\
+    (!ll. destStr (Stream ll) = NONE) /\
+    (!f. destStr (Seq f) = NONE)``,
+  qexists_tac `\f. if f 0 = iNum 1 then SOME (@n. Str n = f) else NONE`
+  \\ fs [] \\ rw [] \\ EVAL_TAC));
+val _ = export_rewrites ["destStr_def"];
+
+val destStr_o_Str = Q.store_thm("destStr_o_Str[simp]",
+  `destStr o Str = SOME`, rw[FUN_EQ_THM]);
+
+val destCons_def = new_specification("destCons_def",["destCons"],prove(``
+  ?destCons.
+    (!n. destCons (Num n) = NONE) /\
+    (!s. destCons (Str s) = NONE) /\
+    (!x y. destCons (Cons x y) = SOME (x,y)) /\
+    (!l. destCons (List l) = NONE) /\
+    (!ll. destCons (Stream ll) = NONE) /\
+    (!f. destCons (Seq f) = NONE)``,
+  qexists_tac `\f. if f 0 = iNum 2 then SOME (@n. Cons (FST n) (SND n) = f) else NONE`
+  \\ fs [] \\ rw [] \\ EVAL_TAC
+  \\ `!n. FST n = x ∧ SND n = y <=> n = (x,y)` by fs [FORALL_PROD]
+  \\ asm_rewrite_tac [] \\ fs []));
+val _ = export_rewrites ["destCons_def"];
+
+val destList_def = new_specification("destList_def",["destList"],prove(``
+  ?destList.
+    (!n. destList (Num n) = NONE) /\
+    (!s. destList (Str s) = NONE) /\
+    (!x y. destList (Cons x y) = NONE) /\
+    (!l. destList (List l) = SOME l) /\
+    (!ll. destList (Stream ll) = NONE) /\
+    (!f. destList (Seq f) = NONE)``,
+  qexists_tac `\f. if f 0 = iNum 3 then SOME (@n. List n = f) else NONE`
+  \\ fs [] \\ rw [] \\ EVAL_TAC));
+val _ = export_rewrites ["destList_def"];
+
+val destStream_def = new_specification("destStream_def",["destStream"],prove(``
+  ?destStream.
+    (!n. destStream (Num n) = NONE) /\
+    (!s. destStream (Str s) = NONE) /\
+    (!x y. destStream (Cons x y) = NONE) /\
+    (!l. destStream (List l) = NONE) /\
+    (!ll. destStream (Stream ll) = SOME ll) /\
+    (!f. destStream (Seq f) = NONE)``,
+  qexists_tac `\f. if f 0 = iNum 4 then SOME (@n. Stream n = f) else NONE`
+  \\ fs [] \\ rw [] \\ EVAL_TAC));
+val _ = export_rewrites ["destStream_def"];
+
+val destSeq_def = new_specification("destSeq_def",["destSeq"],prove(``
+  ?destSeq.
+    (!n. destSeq (Num n) = NONE) /\
+    (!s. destSeq (Str s) = NONE) /\
+    (!x y. destSeq (Cons x y) = NONE) /\
+    (!l. destSeq (List l) = NONE) /\
+    (!ll. destSeq (Stream ll) = NONE) /\
+    (!f. destSeq (Seq f) = SOME f)``,
+  qexists_tac `\f. if f 0 = iNum 5 then SOME (@n. Seq n = f) else NONE`
+  \\ fs [] \\ rw [] \\ EVAL_TAC));
+val _ = export_rewrites ["destSeq_def"];
+
+val encode_pair_def = Define`
+  encode_pair e1 e2 (x,y) = Cons (e1 x) (e2 y)`;
+
+val encode_list_def = Define`
+  encode_list e l = List (MAP e l)`;
+
+(*
+
+val decode_pair_def = Define`
+  (decode_pair d1 d2 (Cons f1 f2) =
+      OPTION_BIND (d1 f1)
+      (λx. OPTION_BIND (d2 f2)
+      (λy. SOME (x,y)))) ∧
+  (decode_pair _ _ _ = NONE)`;
+
+val decode_encode_pair = Q.store_thm(
+  "decode_encode_pair",
+  `(∀x. d1 (e1 x) = SOME x) ∧ (∀y. d2 (e2 y) = SOME y) ⇒
+   ∀p. decode_pair d1 d2 (encode_pair e1 e2 p) = SOME p`,
+  strip_tac >> Cases >> simp[encode_pair_def, decode_pair_def]);
+
+val decode_list_def = Define`
+  (decode_list d (List fs) = OPT_MMAP d fs) ∧
+  (decode_list d _ = NONE)`;
+
+val decode_encode_list = Q.store_thm(
+  "decode_encode_list[simp]",
+  `(∀x. d (e x) = SOME x) ⇒
+   ∀l. decode_list d (encode_list e l) = SOME l`,
+  strip_tac >> simp[decode_list_def, encode_list_def] >> Induct >>
+  simp[OPT_MMAP_def]);
+
+*)
+
+(* make an ffi_next function from base functions and encode/decode *)
+val mk_ffi_next_def = Define`
+  mk_ffi_next (encode,decode,ls) name conf bytes s =
+    OPTION_BIND (ALOOKUP ls name) (λf.
+    OPTION_BIND (decode s) (λs.
+    OPTION_BIND (f conf bytes s) (λ(bytes,s).
+    SOME (bytes,encode s))))`;
+
+val _ = export_theory()
